spec/design/TCB_H.thy
@@ -324,7 +324,6 @@ defs invokeTCB_def:
                 cteDelete bufferSlot True;
                 withoutPreemption $ threadSet
                     (\<lambda> t. t \<lparr>tcbIPCBuffer := ptr\<rparr>) target;
-                withoutPreemption $ asUser target $ setRegister tpidrurwRegister $ fromVPtr ptr;
                 withoutPreemption $ (case frame of
                       Some (newCap, srcSlot) \<Rightarrow>  
                         checkCapAt newCap srcSlot
