spec/design/X64/ArchStateData_H.thy
@@ -23,80 +23,218 @@ imports
   ArchStructures_H
 begin
 
-context X64 begin
+context Arch begin global_naming X64_H
 
 datatype kernel_state =
-    X64KernelState machine_word "asid \<Rightarrow> ((machine_word) option)" machine_word
+    X64KernelState "asid \<Rightarrow> ((machine_word) option)" "asid \<Rightarrow> ((machine_word) option)" machine_word "machine_word list" "machine_word list" "machine_word list"
+
+primrec
+  x64KSGlobalPDs :: "kernel_state \<Rightarrow> machine_word list"
+where
+  "x64KSGlobalPDs (X64KernelState v0 v1 v2 v3 v4 v5) = v4"
+
+primrec
+  x64KSASIDMap :: "kernel_state \<Rightarrow> asid \<Rightarrow> ((machine_word) option)"
+where
+  "x64KSASIDMap (X64KernelState v0 v1 v2 v3 v4 v5) = v1"
 
 primrec
   x64KSASIDTable :: "kernel_state \<Rightarrow> asid \<Rightarrow> ((machine_word) option)"
 where
-  "x64KSASIDTable (X64KernelState v0 v1 v2) = v1"
+  "x64KSASIDTable (X64KernelState v0 v1 v2 v3 v4 v5) = v0"
+
+primrec
+  x64KSGlobalPDPTs :: "kernel_state \<Rightarrow> machine_word list"
+where
+  "x64KSGlobalPDPTs (X64KernelState v0 v1 v2 v3 v4 v5) = v3"
 
 primrec
   x64KSGlobalPML4 :: "kernel_state \<Rightarrow> machine_word"
 where
-  "x64KSGlobalPML4 (X64KernelState v0 v1 v2) = v2"
+  "x64KSGlobalPML4 (X64KernelState v0 v1 v2 v3 v4 v5) = v2"
 
 primrec
-  x64KSGDT :: "kernel_state \<Rightarrow> machine_word"
+  x64KSGlobalPTs :: "kernel_state \<Rightarrow> machine_word list"
 where
-  "x64KSGDT (X64KernelState v0 v1 v2) = v0"
+  "x64KSGlobalPTs (X64KernelState v0 v1 v2 v3 v4 v5) = v5"
+
+primrec
+  x64KSGlobalPDs_update :: "((machine_word list) \<Rightarrow> (machine_word list)) \<Rightarrow> kernel_state \<Rightarrow> kernel_state"
+where
+  "x64KSGlobalPDs_update f (X64KernelState v0 v1 v2 v3 v4 v5) = X64KernelState v0 v1 v2 v3 (f v4) v5"
+
+primrec
+  x64KSASIDMap_update :: "((asid \<Rightarrow> ((machine_word) option)) \<Rightarrow> (asid \<Rightarrow> ((machine_word) option))) \<Rightarrow> kernel_state \<Rightarrow> kernel_state"
+where
+  "x64KSASIDMap_update f (X64KernelState v0 v1 v2 v3 v4 v5) = X64KernelState v0 (f v1) v2 v3 v4 v5"
 
 primrec
   x64KSASIDTable_update :: "((asid \<Rightarrow> ((machine_word) option)) \<Rightarrow> (asid \<Rightarrow> ((machine_word) option))) \<Rightarrow> kernel_state \<Rightarrow> kernel_state"
 where
-  "x64KSASIDTable_update f (X64KernelState v0 v1 v2) = X64KernelState v0 (f v1) v2"
+  "x64KSASIDTable_update f (X64KernelState v0 v1 v2 v3 v4 v5) = X64KernelState (f v0) v1 v2 v3 v4 v5"
+
+primrec
+  x64KSGlobalPDPTs_update :: "((machine_word list) \<Rightarrow> (machine_word list)) \<Rightarrow> kernel_state \<Rightarrow> kernel_state"
+where
+  "x64KSGlobalPDPTs_update f (X64KernelState v0 v1 v2 v3 v4 v5) = X64KernelState v0 v1 v2 (f v3) v4 v5"
 
 primrec
   x64KSGlobalPML4_update :: "(machine_word \<Rightarrow> machine_word) \<Rightarrow> kernel_state \<Rightarrow> kernel_state"
 where
-  "x64KSGlobalPML4_update f (X64KernelState v0 v1 v2) = X64KernelState v0 v1 (f v2)"
+  "x64KSGlobalPML4_update f (X64KernelState v0 v1 v2 v3 v4 v5) = X64KernelState v0 v1 (f v2) v3 v4 v5"
 
 primrec
-  x64KSGDT_update :: "(machine_word \<Rightarrow> machine_word) \<Rightarrow> kernel_state \<Rightarrow> kernel_state"
+  x64KSGlobalPTs_update :: "((machine_word list) \<Rightarrow> (machine_word list)) \<Rightarrow> kernel_state \<Rightarrow> kernel_state"
 where
-  "x64KSGDT_update f (X64KernelState v0 v1 v2) = X64KernelState (f v0) v1 v2"
+  "x64KSGlobalPTs_update f (X64KernelState v0 v1 v2 v3 v4 v5) = X64KernelState v0 v1 v2 v3 v4 (f v5)"
 
 abbreviation (input)
-  X64KernelState_trans :: "(machine_word) \<Rightarrow> (asid \<Rightarrow> ((machine_word) option)) \<Rightarrow> (machine_word) \<Rightarrow> kernel_state" ("X64KernelState'_ \<lparr> x64KSGDT= _, x64KSASIDTable= _, x64KSGlobalPML4= _ \<rparr>")
+  X64KernelState_trans :: "(asid \<Rightarrow> ((machine_word) option)) \<Rightarrow> (asid \<Rightarrow> ((machine_word) option)) \<Rightarrow> (machine_word) \<Rightarrow> (machine_word list) \<Rightarrow> (machine_word list) \<Rightarrow> (machine_word list) \<Rightarrow> kernel_state" ("X64KernelState'_ \<lparr> x64KSASIDTable= _, x64KSASIDMap= _, x64KSGlobalPML4= _, x64KSGlobalPDPTs= _, x64KSGlobalPDs= _, x64KSGlobalPTs= _ \<rparr>")
 where
-  "X64KernelState_ \<lparr> x64KSGDT= v0, x64KSASIDTable= v1, x64KSGlobalPML4= v2 \<rparr> == X64KernelState v0 v1 v2"
+  "X64KernelState_ \<lparr> x64KSASIDTable= v0, x64KSASIDMap= v1, x64KSGlobalPML4= v2, x64KSGlobalPDPTs= v3, x64KSGlobalPDs= v4, x64KSGlobalPTs= v5 \<rparr> == X64KernelState v0 v1 v2 v3 v4 v5"
+
+lemma x64KSGlobalPDs_x64KSGlobalPDs_update [simp]:
+  "x64KSGlobalPDs (x64KSGlobalPDs_update f v) = f (x64KSGlobalPDs v)"
+  by (cases v) simp
+
+lemma x64KSGlobalPDs_x64KSASIDMap_update [simp]:
+  "x64KSGlobalPDs (x64KSASIDMap_update f v) = x64KSGlobalPDs v"
+  by (cases v) simp
+
+lemma x64KSGlobalPDs_x64KSASIDTable_update [simp]:
+  "x64KSGlobalPDs (x64KSASIDTable_update f v) = x64KSGlobalPDs v"
+  by (cases v) simp
+
+lemma x64KSGlobalPDs_x64KSGlobalPDPTs_update [simp]:
+  "x64KSGlobalPDs (x64KSGlobalPDPTs_update f v) = x64KSGlobalPDs v"
+  by (cases v) simp
+
+lemma x64KSGlobalPDs_x64KSGlobalPML4_update [simp]:
+  "x64KSGlobalPDs (x64KSGlobalPML4_update f v) = x64KSGlobalPDs v"
+  by (cases v) simp
+
+lemma x64KSGlobalPDs_x64KSGlobalPTs_update [simp]:
+  "x64KSGlobalPDs (x64KSGlobalPTs_update f v) = x64KSGlobalPDs v"
+  by (cases v) simp
+
+lemma x64KSASIDMap_x64KSGlobalPDs_update [simp]:
+  "x64KSASIDMap (x64KSGlobalPDs_update f v) = x64KSASIDMap v"
+  by (cases v) simp
+
+lemma x64KSASIDMap_x64KSASIDMap_update [simp]:
+  "x64KSASIDMap (x64KSASIDMap_update f v) = f (x64KSASIDMap v)"
+  by (cases v) simp
+
+lemma x64KSASIDMap_x64KSASIDTable_update [simp]:
+  "x64KSASIDMap (x64KSASIDTable_update f v) = x64KSASIDMap v"
+  by (cases v) simp
+
+lemma x64KSASIDMap_x64KSGlobalPDPTs_update [simp]:
+  "x64KSASIDMap (x64KSGlobalPDPTs_update f v) = x64KSASIDMap v"
+  by (cases v) simp
+
+lemma x64KSASIDMap_x64KSGlobalPML4_update [simp]:
+  "x64KSASIDMap (x64KSGlobalPML4_update f v) = x64KSASIDMap v"
+  by (cases v) simp
+
+lemma x64KSASIDMap_x64KSGlobalPTs_update [simp]:
+  "x64KSASIDMap (x64KSGlobalPTs_update f v) = x64KSASIDMap v"
+  by (cases v) simp
+
+lemma x64KSASIDTable_x64KSGlobalPDs_update [simp]:
+  "x64KSASIDTable (x64KSGlobalPDs_update f v) = x64KSASIDTable v"
+  by (cases v) simp
+
+lemma x64KSASIDTable_x64KSASIDMap_update [simp]:
+  "x64KSASIDTable (x64KSASIDMap_update f v) = x64KSASIDTable v"
+  by (cases v) simp
 
 lemma x64KSASIDTable_x64KSASIDTable_update [simp]:
   "x64KSASIDTable (x64KSASIDTable_update f v) = f (x64KSASIDTable v)"
+  by (cases v) simp
+
+lemma x64KSASIDTable_x64KSGlobalPDPTs_update [simp]:
+  "x64KSASIDTable (x64KSGlobalPDPTs_update f v) = x64KSASIDTable v"
   by (cases v) simp
 
 lemma x64KSASIDTable_x64KSGlobalPML4_update [simp]:
   "x64KSASIDTable (x64KSGlobalPML4_update f v) = x64KSASIDTable v"
   by (cases v) simp
 
-lemma x64KSASIDTable_x64KSGDT_update [simp]:
-  "x64KSASIDTable (x64KSGDT_update f v) = x64KSASIDTable v"
+lemma x64KSASIDTable_x64KSGlobalPTs_update [simp]:
+  "x64KSASIDTable (x64KSGlobalPTs_update f v) = x64KSASIDTable v"
+  by (cases v) simp
+
+lemma x64KSGlobalPDPTs_x64KSGlobalPDs_update [simp]:
+  "x64KSGlobalPDPTs (x64KSGlobalPDs_update f v) = x64KSGlobalPDPTs v"
+  by (cases v) simp
+
+lemma x64KSGlobalPDPTs_x64KSASIDMap_update [simp]:
+  "x64KSGlobalPDPTs (x64KSASIDMap_update f v) = x64KSGlobalPDPTs v"
+  by (cases v) simp
+
+lemma x64KSGlobalPDPTs_x64KSASIDTable_update [simp]:
+  "x64KSGlobalPDPTs (x64KSASIDTable_update f v) = x64KSGlobalPDPTs v"
+  by (cases v) simp
+
+lemma x64KSGlobalPDPTs_x64KSGlobalPDPTs_update [simp]:
+  "x64KSGlobalPDPTs (x64KSGlobalPDPTs_update f v) = f (x64KSGlobalPDPTs v)"
+  by (cases v) simp
+
+lemma x64KSGlobalPDPTs_x64KSGlobalPML4_update [simp]:
+  "x64KSGlobalPDPTs (x64KSGlobalPML4_update f v) = x64KSGlobalPDPTs v"
+  by (cases v) simp
+
+lemma x64KSGlobalPDPTs_x64KSGlobalPTs_update [simp]:
+  "x64KSGlobalPDPTs (x64KSGlobalPTs_update f v) = x64KSGlobalPDPTs v"
+  by (cases v) simp
+
+lemma x64KSGlobalPML4_x64KSGlobalPDs_update [simp]:
+  "x64KSGlobalPML4 (x64KSGlobalPDs_update f v) = x64KSGlobalPML4 v"
+  by (cases v) simp
+
+lemma x64KSGlobalPML4_x64KSASIDMap_update [simp]:
+  "x64KSGlobalPML4 (x64KSASIDMap_update f v) = x64KSGlobalPML4 v"
   by (cases v) simp
 
 lemma x64KSGlobalPML4_x64KSASIDTable_update [simp]:
   "x64KSGlobalPML4 (x64KSASIDTable_update f v) = x64KSGlobalPML4 v"
   by (cases v) simp
 
+lemma x64KSGlobalPML4_x64KSGlobalPDPTs_update [simp]:
+  "x64KSGlobalPML4 (x64KSGlobalPDPTs_update f v) = x64KSGlobalPML4 v"
+  by (cases v) simp
+
 lemma x64KSGlobalPML4_x64KSGlobalPML4_update [simp]:
   "x64KSGlobalPML4 (x64KSGlobalPML4_update f v) = f (x64KSGlobalPML4 v)"
   by (cases v) simp
 
-lemma x64KSGlobalPML4_x64KSGDT_update [simp]:
-  "x64KSGlobalPML4 (x64KSGDT_update f v) = x64KSGlobalPML4 v"
+lemma x64KSGlobalPML4_x64KSGlobalPTs_update [simp]:
+  "x64KSGlobalPML4 (x64KSGlobalPTs_update f v) = x64KSGlobalPML4 v"
   by (cases v) simp
 
-lemma x64KSGDT_x64KSASIDTable_update [simp]:
-  "x64KSGDT (x64KSASIDTable_update f v) = x64KSGDT v"
+lemma x64KSGlobalPTs_x64KSGlobalPDs_update [simp]:
+  "x64KSGlobalPTs (x64KSGlobalPDs_update f v) = x64KSGlobalPTs v"
   by (cases v) simp
 
-lemma x64KSGDT_x64KSGlobalPML4_update [simp]:
-  "x64KSGDT (x64KSGlobalPML4_update f v) = x64KSGDT v"
+lemma x64KSGlobalPTs_x64KSASIDMap_update [simp]:
+  "x64KSGlobalPTs (x64KSASIDMap_update f v) = x64KSGlobalPTs v"
   by (cases v) simp
 
-lemma x64KSGDT_x64KSGDT_update [simp]:
-  "x64KSGDT (x64KSGDT_update f v) = f (x64KSGDT v)"
+lemma x64KSGlobalPTs_x64KSASIDTable_update [simp]:
+  "x64KSGlobalPTs (x64KSASIDTable_update f v) = x64KSGlobalPTs v"
+  by (cases v) simp
+
+lemma x64KSGlobalPTs_x64KSGlobalPDPTs_update [simp]:
+  "x64KSGlobalPTs (x64KSGlobalPDPTs_update f v) = x64KSGlobalPTs v"
+  by (cases v) simp
+
+lemma x64KSGlobalPTs_x64KSGlobalPML4_update [simp]:
+  "x64KSGlobalPTs (x64KSGlobalPML4_update f v) = x64KSGlobalPTs v"
+  by (cases v) simp
+
+lemma x64KSGlobalPTs_x64KSGlobalPTs_update [simp]:
+  "x64KSGlobalPTs (x64KSGlobalPTs_update f v) = f (x64KSGlobalPTs v)"
   by (cases v) simp
 
 definition
