spec/design/skel/X64/ArchInterruptDecls_H.thy
@@ -12,9 +12,9 @@ theory ArchInterruptDecls_H
 imports "../RetypeDecls_H" "../CNode_H" 
 begin
 
-context X64 begin
+context Arch begin global_naming X64_H
 
-#INCLUDE_HASKELL SEL4/Object/Interrupt/X64.lhs CONTEXT X64 decls_only ArchInv=ArchRetypeDecls_H Arch=MachineOps
+#INCLUDE_HASKELL SEL4/Object/Interrupt/X64.lhs CONTEXT X64_H decls_only ArchInv=ArchRetypeDecls_H Arch=MachineOps
 
 end (* context X64 *)
 
