spec/design/skel/X64/ArchRetype_H.thy
@@ -18,10 +18,10 @@ imports
   "../KI_Decls_H"
 begin
 
-context X64 begin
+context Arch begin global_naming X64_H
 
-#INCLUDE_HASKELL SEL4/Object/ObjectType/X64.lhs CONTEXT X64 Arch.Types=ArchTypes_H ArchInv=ArchRetypeDecls_H bodies_only
-#INCLUDE_HASKELL SEL4/API/Invocation/X64.lhs CONTEXT X64 bodies_only
+#INCLUDE_HASKELL SEL4/Object/ObjectType/X64.lhs CONTEXT X64_H Arch.Types=ArchTypes_H ArchInv=ArchRetypeDecls_H bodies_only
+#INCLUDE_HASKELL SEL4/API/Invocation/X64.lhs CONTEXT X64_H bodies_only
 
 end (* context X64 *)
 end
