spec/design/skel/X64/ArchThread_H.thy
@@ -18,9 +18,9 @@ imports
 begin
 
 
-context X64 begin
+context Arch begin global_naming X64_H
 
-#INCLUDE_HASKELL SEL4/Kernel/Thread/X64.lhs CONTEXT X64 Arch=MachineOps ArchReg=MachineTypes bodies_only
+#INCLUDE_HASKELL SEL4/Kernel/Thread/X64.lhs CONTEXT X64_H Arch=MachineOps ArchReg=MachineTypes bodies_only
 
 end (* context X64 *)
 
