spec/design/skel/X64/ArchTypes_H.thy
@@ -21,13 +21,66 @@ imports
   "../../../lib/Lib"
 begin
 
-context X64 begin
-
 #INCLUDE_HASKELL SEL4/API/Types/Universal.lhs all_bits
 
-#INCLUDE_HASKELL SEL4/API/Types/X64.lhs CONTEXT X64
-#INCLUDE_HASKELL SEL4/API/Types/X64.lhs CONTEXT X64 instanceproofs 
+context Arch begin global_naming X64_H
 
-end (* context X64 *) 
+#INCLUDE_HASKELL SEL4/API/Types/X64.lhs CONTEXT X64_H
+
+end
+
+text {* object\_type instance proofs *}
+
+qualify X64_H (in Arch)
+instantiation X64_H.object_type :: enum
+begin
+interpretation Arch .
+definition
+  enum_object_type: "enum_class.enum \<equiv>
+    map APIObjectType (enum_class.enum :: apiobject_type list) @
+     [SmallPageObject,
+      LargePageObject,
+      HugePageObject,
+      PageTableObject,
+      PageDirectoryObject,
+      PDPointerTableObject,
+      PageMapL4Object
+    ]"
+
+definition
+  "enum_class.enum_all (P :: object_type \<Rightarrow> bool) \<longleftrightarrow> Ball UNIV P"
+
+definition
+  "enum_class.enum_ex (P :: object_type \<Rightarrow> bool) \<longleftrightarrow> Bex UNIV P"
+
+  instance
+    apply intro_classes
+     apply (safe, simp)
+     apply (case_tac x)
+    apply (simp_all add: enum_object_type)
+    apply (auto intro: distinct_map_enum
+                 simp: enum_all_object_type_def enum_ex_object_type_def)
+    done
+end
+
+
+instantiation X64_H.object_type :: enum_alt
+begin
+interpretation Arch .
+definition
+  enum_alt_object_type: "enum_alt \<equiv>
+    alt_from_ord (enum :: object_type list)"
+instance ..
+end
+
+instantiation X64_H.object_type :: enumeration_both
+begin
+interpretation Arch .
+instance by (intro_classes, simp add: enum_alt_object_type)
+end
+
+context begin interpretation Arch .
+requalify_types object_type
+end
 
 end
