spec/design/skel/X64/Arch_Structs_B.thy
@@ -15,12 +15,12 @@ chapter "Common, Architecture-Specific Data Types"
 theory Arch_Structs_B
 imports "~~/src/HOL/Main" "../../../spec/machine/Setup_Locale"
 begin
-(* FIXME: Clagged from ARM version *)
+(* FIXME: Clagged from X64 version *)
 
 context Arch begin global_naming X64_H
 
 (* FIXME: add an underscore after translation of X64 prefix? *)
-#INCLUDE_HASKELL SEL4/Model/StateData/X64.lhs CONTEXT X64 ONLY X64VSpaceRegionUse
+#INCLUDE_HASKELL SEL4/Model/StateData/X64.lhs CONTEXT X64_H ONLY X64VSpaceRegionUse
 
 end (* context X64 *)
 
