spec/design/skel/X64/State_H.thy
@@ -20,7 +20,7 @@ imports
   RegisterSet_H
   "../../machine/X64/MachineOps"
 begin
-context X64 begin
+context Arch begin global_naming X64_H
 
 definition
   Word :: "machine_word \<Rightarrow> machine_word"
@@ -28,7 +28,7 @@ where
   Word_def[simp]:
  "Word \<equiv> id"
 
-#INCLUDE_HASKELL SEL4/Machine/RegisterSet.lhs Arch=MachineTypes all_bits NOT UserContext UserMonad getRegister setRegister newContext mask Word PPtr
+#INCLUDE_HASKELL SEL4/Machine/RegisterSet.lhs Arch=X64 CONTEXT X64_H all_bits NOT UserContext UserMonad getRegister setRegister newContext mask Word PPtr
 
 definition
   PPtr :: "machine_word \<Rightarrow> machine_word"
@@ -47,5 +47,5 @@ definition
 where
  "nullPointer \<equiv> 0"
 
-end (* context X64 *)
+end
 end
